\documentclass{article}

\usepackage{amsfonts}
\usepackage{graphicx}
\usepackage{amssymb}
\usepackage{amsmath}

\setlength\parindent{18pt}

\begin{document}


Textbook Section 2.3:

13) Separate variables in Eq. (12) and substitute
$u = v \sqrt{\frac{p}{g}}$ to obtain the upward-motion
velocity function given in Eq. (13) with initial condition
$v(0) = v_0$.

Equation 12:

\[\frac{dv}{dt} = -g - pv^2 = -g \left( 1+\frac{p}{g}v^2 \right).\]

Remember:

\[\int \frac{1}{1 + u^2}du = tan^{-1}(u) + C\]

Equation 13:

\[v(t) = \sqrt{\frac{g}{p}}tan(C_1 - t \sqrt{pg})\]

with

\[C_1 = tan^{-1} \left( v_0 \sqrt{\frac{p}{g}} \right).\]



Work:

\[-g \left( 1+\frac{p}{g}v^2 \right)\]
with
\[u = v \sqrt{\frac{p}{g}}\]
\[\implies du = \sqrt{\frac{p}{g}} dv\]
yields:
\[\frac{du}{dt} = -g(1 + u^2)\]
\[\implies \sqrt{\frac{p}{g}} \int \frac{dv}{1 + u^2} = \int -gdt\]
\[\implies \sqrt{\frac{p}{g}} tan^{-1}(u) = -gt + u_0\]
\[\implies tan^{-1}(u) = \sqrt{\frac{p}{g}} \cdot (-gt + u_0)\]
\[\implies tan^{-1}(u)= -\sqrt{pg}t + \sqrt{\frac{p}{g}} u_0\]
\[\implies u = tan \left( \sqrt{\frac{p}{g}} u_0 - \sqrt{pg}t \right) \]
\[v \sqrt{\frac{p}{g}} = tan \left( \sqrt{\frac{p}{g}} u_0 - \sqrt{pg}t \right)\]
\[v = \sqrt{\frac{g}{p}} tan \left( tan^{-1} \left( \sqrt{\frac{p}{g}} v_0 \right) - \sqrt{pg}t \right)\]



14) Integrate the velocity function in Eq. (13) to obtain
the upward-motion function in Eq. (14) with initial
condition $y(0) = y_0$.

Recall:

\[\int tan(u)du = -ln \left| cos(u) \right| + C\]

Equation 14:

\[y(t) = y_0 + \frac{1}{p}ln \left| \frac{cos(C_1 - t \sqrt{pg})}{cos(C_1)} \right| \]



Work:

\[\frac{dy}{dt} = \sqrt{\frac{g}{p}} tan \left( C1 - \sqrt{pg}t \right)\]

Let $u = C1 - \sqrt{pg}t$.
$\implies du = -\sqrt{pg} dt$.


\[\implies \frac{dy}{du} = -\sqrt{\frac{g}{p}} tan(u)\]
\[\implies dy = -\sqrt{\frac{g}{p}} tan(u) du\]
\[-\sqrt{\frac{p}{g}} dy = tan(u) du\]
\[-\sqrt{\frac{p}{g}} \int dy = \int tan(u) du\]
\[-\sqrt{\frac{p}{g}} y = -ln \left| cos(u) \right| + u_0\]
\[y = \frac{g}{p} (-u_0 + ln \left| cos(u) \right|)\]
Since $y(0) = y_0$, then the inside of $ln$ must be $1$.
And since $cos(C1 - \sqrt{pg}t)$ at $t = 0$ is $C1$,
we have to divide it out.
\[y = y_0 + \frac{g}{p} \left( ln \left| \frac{cos(C1 - \sqrt{pg}t)}{cos(C_1)} \right| \right)\]

Not sure how $\frac{g}{p}$ is supposed to become $\frac{1}{p}$.



Textbook Section 2.4:

4) $y' = x - y, y(0) = 1; y(x) = 2e^{-x} + x - 1$

For euler's method with step size of 0.25:
We get an approximation of y at 0.5 of $0.625$.

For euler's method with step size of 0.1:
We get an approximation of y at 0.5 of $0.681$.

The actual value of y at 0.5 is $0.713$.


Textbook Section 2.5:

4) $y' = x - y, y(0) = 1; y(x) = 2e^{-x} + x - 1$

\begin{center}
\begin{tabular}{ c c c }
    x & approximation & actual \\
    0.1 & 0.9100 & 0.9097 \\
    0.2 & 0.8381 & 0.8375 \\
    0.3 & 0.7824 & 0.7816 \\
    0.4 & 0.7416 & 0.7406 \\
    0.5 & 0.7142 & 0.7131
\end{tabular}
\end{center}



Textbook Section 2.6:

4) $y' = x - y, y(0) = 1; y(x) = 2e^{-x} + x - 1$

\begin{center}
\begin{tabular}{ c c c }
    x & approximation & actual \\
    0.25 & 0.80762 & 0.80762 \\
    0.5 & 0.71309 & 0.71306
\end{tabular}
\end{center}




\end{document}
